terms.v
@@ -184,24 +184,27 @@ https://coq.inria.fr/bugs/show_bug.cgi?id=3343
    *) 
 
 (* --- variables --- *)
-Fixpoint free_vars {NVar VarClass} `{VarType NVar VarClass} {gts : GenericTermSig}  
+
+(** Just decidability of equality on variables suffices for these definitions.
+  The full [VarType] may not be needed until [ssubst]*)
+Fixpoint free_vars {NVar} `{Deq NVar} {gts : GenericTermSig}  
   (t:NTerm) {struct t}: list NVar :=
   match t with
   | vterm v => [v]
-  | oterm op bts => flat_map (@free_vars_bterm NVar _ _ _ _)  bts
+  | oterm op bts => flat_map (@free_vars_bterm NVar _ _)  bts
   end
- with free_vars_bterm {NVar VarClass} `{VarType NVar VarClass} {gts : GenericTermSig}  (bt : BTerm)
+ with free_vars_bterm {NVar} `{Deq NVar} {gts : GenericTermSig}  (bt : BTerm)
   {struct bt} : list NVar :=
   match bt with
   | bterm  lv nt => remove_nvars lv (free_vars nt)
   end.
 
-Fixpoint bound_vars {NVar VarClass} `{VarType NVar VarClass} {gts : GenericTermSig} (t : NTerm) : list NVar :=
+Fixpoint bound_vars {NVar} `{Deq NVar} {gts : GenericTermSig} (t : NTerm) : list NVar :=
   match t with
   | vterm v => []
-  | oterm op bts => flat_map (@bound_vars_bterm NVar VarClass _ _ _ _)  bts
+  | oterm op bts => flat_map (@bound_vars_bterm NVar _ _ _)  bts
   end
- with bound_vars_bterm {NVar VarClass} `{VarType NVar VarClass} {gts : GenericTermSig} {gts : GenericTermSig} (bt : BTerm ) 
+ with bound_vars_bterm {NVar} `{Deq NVar} {gts : GenericTermSig} {gts : GenericTermSig} (bt : BTerm ) 
   :list NVar :=
   match bt with
   | bterm lv nt => lv ++ bound_vars nt
